memes tipos de carinhas sao

FpInLean/Chap10.lean
@@ -36,11 +36,129 @@ def NonTail.factorial : Nat → Nat
   | n + 1 => factorial n * (n + 1)
 
 def Tail.factorialHelper (acc : Nat) : Nat → Nat
-  | 0 => 1 * acc
-  | 5 => 2
-  | n + 1 => Tail.factorialHelper (acc * n) n
+  | 0 => acc
+  | n + 1 => Tail.factorialHelper (acc * (n + 1)) n
 
-def Tail.factorial (x : Nat) : Nat := Tail.factorialHelper x x
+def Tail.factorial : Nat → Nat := Tail.factorialHelper 1
 
 #eval NonTail.factorial 5
 #eval Tail.factorial 5
+
+def NonTail.filter (p : α → Bool) : List α → List α
+  | [] => []
+  | x :: xs =>
+    if p x then
+      x :: filter p xs
+    else
+      filter p xs
+
+def Tail.filterHelper (acc : List α) (f : α → Bool) : List α → List α
+  | [] => acc
+  | x :: xs => let acc₁ := if f x then acc ++ [x] else acc
+               Tail.filterHelper acc₁ f xs
+
+def Tail.filter : (α → Bool) → List α → List α := Tail.filterHelper []
+
+def Nat.even :=
+  fun
+    | Nat.zero => true
+    | Nat.succ x => not (even x)
+
+#eval Tail.filter Nat.even [1, 2, 3, 4, 5]
+
+theorem non_tail_sum_eq_helper_accum (xs : List Nat) :
+  (n : Nat) → n + NonTail.sum xs = Tail.sumHelper n xs := by
+  induction xs with
+  | nil => intro n
+           rfl
+  | cons y ys ih =>
+    intro n
+    simp [NonTail.sum, Tail.sumHelper]
+    rw [←Nat.add_assoc, Nat.add_comm y n]
+    exact ih (n + y)
+
+theorem non_tail_sum_eq_tail_sum : NonTail.sum = Tail.sum := by
+  funext xs
+  simp [Tail.sum]
+  rw [←Nat.zero_add (NonTail.sum xs)]
+  exact non_tail_sum_eq_helper_accum xs 0
+
+theorem zero_add (n : Nat) : 0 + n = n := by
+  induction n with
+  | zero => rfl
+  | succ m =>
+    simp [Add.add]
+
+theorem succ_add : ∀ (x y : Nat), (Nat.succ x) + y = x + (Nat.succ y)
+  | _, 0 => by rfl
+  | n, m + 1 => congrArg Nat.succ (succ_add n m)
+
+theorem succ_add_rev : ∀ (x y : Nat), Nat.succ (x + y) = Nat.succ x + y
+  | _, 0 => by rfl
+  | n, m + 1 => congrArg Nat.succ (succ_add_rev n m)
+
+theorem add_succ (n m : Nat) : n + Nat.succ m = Nat.succ (n + m) := by rfl
+
+theorem add_assoc : ∀ (x y z : Nat), (x + y) + z = x + (y + z) := by
+  intro x
+  induction x with
+  | zero =>
+    intro y
+    intro z
+    rw [zero_add (y + z), zero_add y]
+  | succ m ih =>
+    intro y
+    intro z
+    simp [succ_add]
+    rw [succ_add_rev]
+    exact ih (Nat.succ y) z
+
+theorem add_comm : ∀ (x y : Nat), x + y = y + x := by
+  intro x
+  induction x with
+  | zero =>
+    simp [zero_add]
+  | succ x₁ ih =>
+    intro y
+    simp [succ_add]
+    rw [←succ_add y x₁]
+    exact ih (Nat.succ y)
+
+#eval NonTail.reverse [1, 2, 3, 4]
+#eval Tail.reverse [1, 2, 3, 4]
+
+theorem tail_reverse_eq_helper_accum (xs : List α) :
+  ∀ (xs₁ : List α), NonTail.reverse xs ++ xs₁ = Tail.reverseHelper xs₁ xs := by
+  induction xs with
+  | nil =>
+    intro x
+    rfl
+
+  | cons x xs₁ ih =>
+    intro xs₂
+    simp [NonTail.reverse, Tail.reverseHelper, List.append_assoc]
+    exact ih (x :: xs₂)
+
+theorem non_tail_reverse_eq_tail_reverse : @NonTail.reverse = @Tail.reverse := by
+  funext α xs
+  simp [Tail.reverse]
+  rw [←List.append_nil (NonTail.reverse xs)]
+  exact tail_reverse_eq_helper_accum xs []
+
+theorem factorial_eq_helper_accum (x : Nat) :
+  ∀ (y : Nat), NonTail.factorial x * y = Tail.factorialHelper y x := by
+  induction x with
+  | zero =>
+    intro y
+    simp [NonTail.factorial, Tail.factorialHelper]
+  | succ x₁ ih =>
+    intro y
+    simp [NonTail.factorial, Tail.factorialHelper]
+    rw [Nat.mul_assoc, Nat.mul_comm y (x₁ + 1)]
+    exact ih ((x₁ + 1) * y)
+
+theorem non_tail_factorial_eq_tail_factorial : NonTail.factorial = Tail.factorial := by
+  funext x
+  simp [Tail.factorial]
+  rw [←Nat.one_mul (NonTail.factorial x), Nat.mul_comm]
+  exact factorial_eq_helper_accum x 1
