FpInLean/Chap10/Arrays.lean
@@ -1,0 +1,81 @@
+inductive IsThree : Nat → Prop where
+  | isThree : IsThree 3
+
+theorem four_le_seven : 4 ≤ 7 :=
+  open Nat.le in
+  (step (step (step refl)))
+
+def arrayMapHelper (f : α → β) (arr : Array α) (soFar : Array β) (i : Nat) : Array β :=
+  if inBounds : i < arr.size then
+    arrayMapHelper f arr (soFar.push (f arr[i])) (i + 1)
+  else
+    soFar
+termination_by arrayMapHelper _ arr _ i _ => arr.size - i
+
+def Array.map' (f : α → β) (arr : Array α) : Array β :=
+  arrayMapHelper f arr Array.empty 0
+
+def findHelper (arr : Array α) (p : α → Bool) (i : Nat) : Option (Nat × α) :=
+  if h : i < arr.size then
+    let x := arr[i]
+    if p x then
+      some (i, x)
+    else
+      findHelper arr p (i + 1)
+  else none
+termination_by findHelper arr _ i => arr.size - i
+
+def Array.find' (arr : Array α) (p : α → Bool) : Option (Nat × α) :=
+  findHelper arr p 0
+
+def forMHelper [Monad m] (i : Nat) (arr : Array α) (f : α → m PUnit) : m PUnit :=
+  if h : i < arr.size then do
+    f arr[i]
+    forMHelper (i + 1) arr f
+  else
+    pure ()
+termination_by forMHelper i arr f => arr.size - i
+
+def Array.forM' [Monad m] : Array α → (α → m PUnit) → m PUnit :=
+  forMHelper 0
+
+def reverseHelper (acc : Array α) (i : Nat) (xs : Array α) : Array α :=
+  match i with
+    | Nat.zero => acc
+    | Nat.succ index =>
+      if h : index < xs.size then
+        reverseHelper (acc.push xs[index]) index xs
+      else
+        acc
+
+def Array.reverse' (xs : Array α) : Array α :=
+  reverseHelper Array.empty xs.size xs
+
+#eval #[1, 2, 3, 4].reverse'
+
+def Array.map'' (f : α → β) (xs : Array α) : Array β := Id.run do
+  let mut ys := #[]
+  for x in xs do
+    ys := ys.push (f x)
+  return ys
+
+def Array.find'' (f : α → Bool) (xs : Array α) : Option (Nat × α) := Id.run do
+  let mut i := 0
+  for x in xs do
+    if f x then
+      return some (i, x)
+    else
+      i := i + 1
+  return none
+
+def Array.forM'' [Monad m] (xs : Array α) (f : α → m PUnit) : m PUnit := do
+  for x in xs do
+    f x
+
+def Array.reverse'' (xs : Array α) : Array α := Id.run do
+  let mut ys := #[]
+  for x in xs do
+    ys := #[x] ++ ys
+  return ys
+
+#eval #[1, 2, 3, 4].reverse''
